user 3, session 11016, part 3

diffs-annotated/3/user-3-session-11016.v
@@ -6,16 +6,6 @@ Set Printing Depth 50.
 Remove Search Blacklist "Private_" "_subproof".
 Add Search Blacklist "Private_" "_subproof".
 Require Export LF.Induction.
-Redirect "/var/folders/5x/1mdbpbjd7012l971fq0zkj2w0000gn/T/coqlLYvyf"
-Print Ltac Signatures.
-Timeout 1 Print Grammar tactic.
-Add Search Blacklist "Raw" "Proofs".
-Set Search Output Name Only.
-Redirect "/var/folders/5x/1mdbpbjd7012l971fq0zkj2w0000gn/T/coquLOj9K"
-SearchPattern _.
-Remove Search Blacklist "Raw" "Proofs".
-Unset Search Output Name Only.
-Timeout 1 Print LoadPath.
 Module NatList.
 Inductive natprod : Type :=
     pair : nat -> nat -> natprod.
@@ -23,81 +13,212 @@ Check pair 3 5.
 Definition fst (p : natprod) : nat := match p with
                                       | pair x y => x
                                       end.
-Redirect "/var/folders/5x/1mdbpbjd7012l971fq0zkj2w0000gn/T/coqE4Ezr4"
-Print Ltac Signatures.
-Timeout 1 Print Grammar tactic.
-Add Search Blacklist "Raw" "Proofs".
-Set Search Output Name Only.
-Redirect "/var/folders/5x/1mdbpbjd7012l971fq0zkj2w0000gn/T/coqCzk5aL"
-SearchPattern _.
-Remove Search Blacklist "Raw" "Proofs".
-Unset Search Output Name Only.
 Definition snd (p : natprod) : nat := match p with
                                       | pair x y => y
                                       end.
-Redirect "/var/folders/5x/1mdbpbjd7012l971fq0zkj2w0000gn/T/coqCrPZ4R"
-Print Ltac Signatures.
-Timeout 1 Print Grammar tactic.
-Add Search Blacklist "Raw" "Proofs".
-Set Search Output Name Only.
-Redirect "/var/folders/5x/1mdbpbjd7012l971fq0zkj2w0000gn/T/coq7j3kjf"
-SearchPattern _.
-Remove Search Blacklist "Raw" "Proofs".
-Unset Search Output Name Only.
 Eval vm_compute in fst (pair 3 5).
 Notation "( x , y )" := (pair x y).
 Eval vm_compute in fst (3, 5).
 Definition fst' (p : natprod) : nat := match p with
                                        | (x, y) => x
                                        end.
-Redirect "/var/folders/5x/1mdbpbjd7012l971fq0zkj2w0000gn/T/coq2bhqrC"
-Print Ltac Signatures.
-Timeout 1 Print Grammar tactic.
-Add Search Blacklist "Raw" "Proofs".
-Set Search Output Name Only.
-Redirect "/var/folders/5x/1mdbpbjd7012l971fq0zkj2w0000gn/T/coqpYItQv"
-SearchPattern _.
-Remove Search Blacklist "Raw" "Proofs".
-Unset Search Output Name Only.
 Definition snd' (p : natprod) : nat := match p with
                                        | (x, y) => y
                                        end.
-Redirect "/var/folders/5x/1mdbpbjd7012l971fq0zkj2w0000gn/T/coq1quQMD"
-Print Ltac Signatures.
-Timeout 1 Print Grammar tactic.
-Add Search Blacklist "Raw" "Proofs".
-Set Search Output Name Only.
-Redirect "/var/folders/5x/1mdbpbjd7012l971fq0zkj2w0000gn/T/coqJmXYvc"
-SearchPattern _.
-Remove Search Blacklist "Raw" "Proofs".
-Unset Search Output Name Only.
 Definition swap_pair (p : natprod) : natprod :=
   match p with
   | (x, y) => (y, x)
   end.
-Redirect "/var/folders/5x/1mdbpbjd7012l971fq0zkj2w0000gn/T/coqHKUpla"
-Print Ltac Signatures.
-Timeout 1 Print Grammar tactic.
-Add Search Blacklist "Raw" "Proofs".
-Set Search Output Name Only.
-Redirect "/var/folders/5x/1mdbpbjd7012l971fq0zkj2w0000gn/T/coqsOPX3h"
-SearchPattern _.
-Remove Search Blacklist "Raw" "Proofs".
-Unset Search Output Name Only.
 Theorem surjective_pairing' :
   forall n m : nat, (n, m) = (fst (n, m), snd (n, m)).
 Proof.
 reflexivity.
-Add Search Blacklist "Raw" "Proofs".
-Set Search Output Name Only.
-Redirect "/var/folders/5x/1mdbpbjd7012l971fq0zkj2w0000gn/T/coqdF8onM"
-SearchPattern _.
-Remove Search Blacklist "Raw" "Proofs".
-Unset Search Output Name Only.
 Qed.
 Theorem surjective_pairing_stuck : forall p : natprod, p = (fst p, snd p).
 Proof.
 (simpl).
 Abort.
+Theorem surjective_pairing : forall p : natprod, p = (fst p, snd p).
+Proof.
+(intros p).
+(destruct p as [n m]).
+(simpl).
+reflexivity.
+Qed.
 Theorem snd_fst_is_swap : forall p : natprod, (snd p, fst p) = swap_pair p.
+Proof.
+Redirect "/var/folders/5x/1mdbpbjd7012l971fq0zkj2w0000gn/T/coqjo1a2t"
+Print Ltac Signatures.
+Timeout 1 Print Grammar tactic.
+Add Search Blacklist "Raw" "Proofs".
+Set Search Output Name Only.
+Redirect "/var/folders/5x/1mdbpbjd7012l971fq0zkj2w0000gn/T/coqoemFZB"
+SearchPattern _.
+Remove Search Blacklist "Raw" "Proofs".
+Unset Search Output Name Only.
+Timeout 1 Print LoadPath.
+(destruct p as [n m]).
+(simpl).
+reflexivity.
+Add Search Blacklist "Raw" "Proofs".
+Set Search Output Name Only.
+Redirect "/var/folders/5x/1mdbpbjd7012l971fq0zkj2w0000gn/T/coqoAeqEL"
+SearchPattern _.
+Remove Search Blacklist "Raw" "Proofs".
+Unset Search Output Name Only.
+Qed.
+Theorem fst_swap_is_snd : forall p : natprod, fst (swap_pair p) = snd p.
+Proof.
+(destruct p as [n m]).
+(simpl).
+reflexivity.
+Add Search Blacklist "Raw" "Proofs".
+Set Search Output Name Only.
+Redirect "/var/folders/5x/1mdbpbjd7012l971fq0zkj2w0000gn/T/coqQZNFc3"
+SearchPattern _.
+Remove Search Blacklist "Raw" "Proofs".
+Unset Search Output Name Only.
+Qed.
+Inductive natlist : Type :=
+  | nil : natlist
+  | cons : nat -> natlist -> natlist.
+Redirect "/var/folders/5x/1mdbpbjd7012l971fq0zkj2w0000gn/T/coqglLWz9"
+Print Ltac Signatures.
+Timeout 1 Print Grammar tactic.
+Add Search Blacklist "Raw" "Proofs".
+Set Search Output Name Only.
+Redirect "/var/folders/5x/1mdbpbjd7012l971fq0zkj2w0000gn/T/coq19vlI9"
+SearchPattern _.
+Remove Search Blacklist "Raw" "Proofs".
+Unset Search Output Name Only.
+Definition mylist := cons 1 (cons 2 (cons 3 nil)).
+Notation "x :: l" := (cons x l) (at level 60, right associativity).
+Notation "[ ]" := nil.
+Notation "[ x ; .. ; y ]" := (cons x .. (cons y nil) ..).
+Redirect "/var/folders/5x/1mdbpbjd7012l971fq0zkj2w0000gn/T/coq0uIgCx"
+Print Ltac Signatures.
+Timeout 1 Print Grammar tactic.
+Add Search Blacklist "Raw" "Proofs".
+Set Search Output Name Only.
+Redirect "/var/folders/5x/1mdbpbjd7012l971fq0zkj2w0000gn/T/coqZ5O4Re"
+SearchPattern _.
+Remove Search Blacklist "Raw" "Proofs".
+Unset Search Output Name Only.
+Definition mylist1 := 1 :: 2 :: 3 :: nil.
+Redirect "/var/folders/5x/1mdbpbjd7012l971fq0zkj2w0000gn/T/coqSJdzVM"
+Print Ltac Signatures.
+Timeout 1 Print Grammar tactic.
+Add Search Blacklist "Raw" "Proofs".
+Set Search Output Name Only.
+Redirect "/var/folders/5x/1mdbpbjd7012l971fq0zkj2w0000gn/T/coq5Zg3PD"
+SearchPattern _.
+Remove Search Blacklist "Raw" "Proofs".
+Unset Search Output Name Only.
+Definition mylist2 := 1 :: 2 :: 3 :: nil.
+Definition mylist3 := [1; 2; 3].
+Redirect "/var/folders/5x/1mdbpbjd7012l971fq0zkj2w0000gn/T/coqBGERh0"
+Print Ltac Signatures.
+Timeout 1 Print Grammar tactic.
+Add Search Blacklist "Raw" "Proofs".
+Set Search Output Name Only.
+Redirect "/var/folders/5x/1mdbpbjd7012l971fq0zkj2w0000gn/T/coqBGkalG"
+SearchPattern _.
+Remove Search Blacklist "Raw" "Proofs".
+Unset Search Output Name Only.
+Fixpoint repeat (n count : nat) : natlist :=
+  match count with
+  | O => nil
+  | S count' => n :: repeat n count'
+  end.
+Redirect "/var/folders/5x/1mdbpbjd7012l971fq0zkj2w0000gn/T/coqbnY9WH"
+Print Ltac Signatures.
+Timeout 1 Print Grammar tactic.
+Add Search Blacklist "Raw" "Proofs".
+Set Search Output Name Only.
+Redirect "/var/folders/5x/1mdbpbjd7012l971fq0zkj2w0000gn/T/coqnFbxs3"
+SearchPattern _.
+Remove Search Blacklist "Raw" "Proofs".
+Unset Search Output Name Only.
+Fixpoint length (l : natlist) : nat :=
+  match l with
+  | nil => O
+  | h :: t => S (length t)
+  end.
+Redirect "/var/folders/5x/1mdbpbjd7012l971fq0zkj2w0000gn/T/coqS3p7nv"
+Print Ltac Signatures.
+Timeout 1 Print Grammar tactic.
+Add Search Blacklist "Raw" "Proofs".
+Set Search Output Name Only.
+Redirect "/var/folders/5x/1mdbpbjd7012l971fq0zkj2w0000gn/T/coqtJjrud"
+SearchPattern _.
+Remove Search Blacklist "Raw" "Proofs".
+Unset Search Output Name Only.
+Fixpoint app (l1 l2 : natlist) : natlist :=
+  match l1 with
+  | nil => l2
+  | h :: t => h :: app t l2
+  end.
+Redirect "/var/folders/5x/1mdbpbjd7012l971fq0zkj2w0000gn/T/coqXJy0Pa"
+Print Ltac Signatures.
+Timeout 1 Print Grammar tactic.
+Add Search Blacklist "Raw" "Proofs".
+Set Search Output Name Only.
+Redirect "/var/folders/5x/1mdbpbjd7012l971fq0zkj2w0000gn/T/coqmmf28h"
+SearchPattern _.
+Remove Search Blacklist "Raw" "Proofs".
+Unset Search Output Name Only.
+Notation "x ++ y" := (app x y) (right associativity, at level 60).
+Example test_app1 : [1; 2; 3] ++ [4; 5] = [1; 2; 3; 4; 5].
+Proof.
+reflexivity.
+Qed.
+Example test_app2 : nil ++ [4; 5] = [4; 5].
+Proof.
+reflexivity.
+Qed.
+Example test_app3 : [1; 2; 3] ++ nil = [1; 2; 3].
+Proof.
+reflexivity.
+Qed.
+Definition hd (default : nat) (l : natlist) : nat :=
+  match l with
+  | nil => default
+  | h :: t => h
+  end.
+Redirect "/var/folders/5x/1mdbpbjd7012l971fq0zkj2w0000gn/T/coqSi5oIm"
+Print Ltac Signatures.
+Timeout 1 Print Grammar tactic.
+Add Search Blacklist "Raw" "Proofs".
+Set Search Output Name Only.
+Redirect "/var/folders/5x/1mdbpbjd7012l971fq0zkj2w0000gn/T/coqjbve1B"
+SearchPattern _.
+Remove Search Blacklist "Raw" "Proofs".
+Unset Search Output Name Only.
+Definition tl (l : natlist) : natlist :=
+  match l with
+  | nil => nil
+  | h :: t => t
+  end.
+Redirect "/var/folders/5x/1mdbpbjd7012l971fq0zkj2w0000gn/T/coqkEwuOj"
+Print Ltac Signatures.
+Timeout 1 Print Grammar tactic.
+Add Search Blacklist "Raw" "Proofs".
+Set Search Output Name Only.
+Redirect "/var/folders/5x/1mdbpbjd7012l971fq0zkj2w0000gn/T/coqbK4Fkh"
+SearchPattern _.
+Remove Search Blacklist "Raw" "Proofs".
+Unset Search Output Name Only.
+Example test_hd1 : hd 0 [1; 2; 3] = 1.
+Proof.
+reflexivity.
+Qed.
+Example test_hd2 : hd 0 [ ] = 0.
+Proof.
+reflexivity.
+Qed.
+Example test_tl : tl [1; 2; 3] = [2; 3].
+Proof.
+reflexivity.
+Qed.
+Fixpoint nonzeros (l : natlist) : natlist.
 Proof.
